proof/invariant-abstract/ARM/ArchAInvsPre.thy
@@ -202,7 +202,7 @@ named_theorems AInvsPre_asms
 
 
 lemma (* ptable_rights_imp_frame *)[AInvsPre_asms]:
-  assumes "valid_state s" "canonical_address x"
+  assumes "valid_state s"
   shows "ptable_rights t s x \<noteq> {} \<Longrightarrow>
          ptable_lift t s x = Some (addrFromPPtr y) \<Longrightarrow>
          in_user_frame y s \<or> in_device_frame y s"
