proof/invariant-abstract/Invariants_AI.thy
@@ -45,7 +45,6 @@ requalify_consts
 
   ASIDPoolObj
 
-  canonical_address
   vs_lookup1
   vs_lookup_trans
   vs_refs
